Test HOL_STRING_TYPE support more thoroughly

translator/ml_translator_testScript.sml
@@ -370,4 +370,222 @@ val res = translate TAKE_def;
 val res = translate DROP_def;
 val res = translate chop_str_def
 
+(* translate tricky parts of StringProg *)
+
+val _ = use_string_type false;
+
+val _ = ml_prog_update (add_dec
+  ``Dtabbrev unknown_loc [] "string" (Atapp [] (Short "string"))`` I);
+
+fun get_module_prefix () = let
+  val mods = ml_progLib.get_open_modules (get_ml_prog_state ())
+  in case mods of [] => ""
+    | (m :: ms) => m ^ "_"
+  end
+
+fun trans ml_name rhs = let
+  val prefix = get_module_prefix ()
+  val hol_name = prefix ^ pick_name ml_name
+  val hol_name_clashes = (fst (dest_const rhs) = hol_name)
+                         handle HOL_ERR _ => false
+  val tm = mk_eq(mk_var(hol_name,type_of rhs),rhs)
+  val def = Define `^tm`
+  val _ = (next_ml_names := [ml_name])
+  val v_thm = translate (def |> SIMP_RULE std_ss [FUN_EQ_THM])
+  val v_thm = v_thm |> REWRITE_RULE [def]
+                    |> CONV_RULE (DEPTH_CONV ETA_CONV)
+  val v_name = v_thm |> concl |> rand |> dest_const |> fst
+  val _ = if hol_name_clashes
+          then remove_ovl_mapping hol_name
+                 {Name = hol_name, Thy = current_theory()}
+          else ()
+  (* evaluate precondition *)
+  val pat = PRECONDITION_def |> SPEC_ALL |> GSYM |> concl |> rand
+  fun PRECOND_CONV c tm =
+    if can (match_term pat) tm then RAND_CONV c tm else NO_CONV tm
+  val v_thm = v_thm |> DISCH_ALL
+                    |> CONV_RULE (ONCE_DEPTH_CONV (PRECOND_CONV EVAL))
+                    |> UNDISCH_ALL
+  val _ = save_thm(v_name ^ "_thm",v_thm)
+  in v_thm end
+
+val _ = trans "sub" mlstringSyntax.strsub_tm;
+val _ = trans "implode" mlstringSyntax.implode_tm;
+val _ = trans "explode" mlstringSyntax.explode_tm;
+val _ = trans "size" mlstringSyntax.strlen_tm;
+val _ = trans "concat" mlstringSyntax.concat_tm;
+val _ = trans "substring" mlstringSyntax.substring_tm;
+val result = translate mlstringTheory.strcat_def;
+val _ = trans "^" mlstringSyntax.strcat_tm;
+
+val _ = translate arithmeticTheory.MIN_DEF
+val result = translate (mlstringTheory.extract_def |> REWRITE_RULE [mlstringTheory.implode_def]);
+
+val extract_side_def = definition"extract_side_def";
+val extract_side_thm = Q.prove(
+  `!s i opt. extract_side s i opt`,
+  rw [extract_side_def, arithmeticTheory.MIN_DEF] ) |> update_precondition
+
+val _ = ml_prog_update open_local_block;
+val res = translate (mlstringTheory.concatWith_aux_def |> REWRITE_RULE [mlstringTheory.implode_def]);
+val _ = ml_prog_update open_local_in_block;
+
+val _ = next_ml_names := ["concatWith"];
+val result = translate mlstringTheory.concatWith_def;
+
+val result = translate mlstringTheory.str_def;
+
+val _ = ml_prog_update open_local_block;
+val result = translate mlstringTheory.translate_aux_def;
+val translate_aux_side_def = theorem"translate_aux_side_def";
+val _ = ml_prog_update open_local_in_block;
+
+val _ = next_ml_names := ["translate"];
+val result = translate mlstringTheory.translate_def;
+val translate_side_def = definition"translate_side_def";
+
+val translate_aux_side_thm = Q.prove (
+  `!f s n len. n + len = strlen s ==> translate_aux_side f s n len`,
+  Induct_on `len` \\ rw[Once translate_aux_side_def]);
+
+val translate_side_thm = Q.prove (
+  `!f s. translate_side f s`,
+  rw [translate_side_def, translate_aux_side_thm] ) |> update_precondition
+
+val _ = ml_prog_update open_local_block;
+val r = translate mlstringTheory.splitl_aux_def;
+val _ = ml_prog_update open_local_in_block;
+
+val _ = next_ml_names := ["split"];
+val r = translate mlstringTheory.splitl_def;
+
+val _ = ml_prog_update open_local_block;
+val res = translate mlstringTheory.tokens_aux_def; (* problem *)
+val tokens_aux_side_def = theorem"tokens_aux_side_def";
+val _ = ml_prog_update open_local_in_block;
+
+val _ = next_ml_names := ["tokens"];
+val result = translate mlstringTheory.tokens_def;
+val tokens_side_def = definition"tokens_side_def";
+
+val tokens_aux_side_thm = Q.prove (
+  `!f s ss n len. n + len = strlen s ==> tokens_aux_side f s ss n len`,
+  Induct_on `len` \\ rw [Once tokens_aux_side_def]);
+
+val tokens_side_thm = Q.prove (
+  `!f s. tokens_side f s`,
+  rw [tokens_side_def, tokens_aux_side_thm] ) |> update_precondition
+
+val _ = ml_prog_update open_local_block;
+val result = translate mlstringTheory.fields_aux_def;
+val fields_aux_side_def = theorem"fields_aux_side_def";
+val _ = ml_prog_update open_local_in_block;
+
+val _ = next_ml_names := ["fields"];
+val result = translate mlstringTheory.fields_def;
+val fields_side_def = definition"fields_side_def";
+
+val fields_aux_side_thm = Q.prove (
+  `!f s ss n len. n + len = strlen s ==> fields_aux_side f s ss n len`,
+  Induct_on `len` \\ rw [Once fields_aux_side_def]);
+
+val fields_side_thm = Q.prove (
+  `!f s. fields_side f s`,
+  rw [fields_side_def, fields_aux_side_thm] ) |> update_precondition
+
+val _ = ml_prog_update open_local_block;
+val result = translate mlstringTheory.isStringThere_aux_def;
+val isStringThere_aux_side_def = theorem"isstringthere_aux_side_def";
+val _ = ml_prog_update open_local_in_block;
+
+val isStringThere_aux_side_thm = Q.prove (
+  `!s1 s2 s1i s2i len.
+     s1i + len ≤ strlen s1 ∧ s2i + len <= strlen s2 ==>
+     isstringthere_aux_side s1 s2 s1i s2i len`,
+  Induct_on `len` \\ rw [Once isStringThere_aux_side_def]);
+
+val _ = next_ml_names := ["isSubstring"];
+val result = translate mlstringTheory.isSubstring_aux_def;
+val isSubstring_aux_side_def = theorem"issubstring_aux_side_def";
+val isSubstring_aux_side_thm = Q.prove (
+  `!s1 s2 lens1 n len.
+    (lens1 = strlen s1) ∧ n + len + lens1 ≤ strlen s2 + 1 ==>
+    issubstring_aux_side s1 s2 lens1 n len`,
+  Induct_on `len` >>
+  rw [Once isSubstring_aux_side_def] >>
+  irule isStringThere_aux_side_thm >> simp[]);
+
+val _ = next_ml_names := ["isSubstring"];
+val result = translate mlstringTheory.isSubstring_def;
+val isSubstring_side_def = definition"issubstring_side_def";
+val isSubstring_side_thm = Q.prove (
+  `!s1 s2. issubstring_side s1 s2`,
+  rw [isSubstring_side_def, isSubstring_aux_side_thm]) |> update_precondition
+
+val _ = next_ml_names := ["isSuffix"];
+val result = translate mlstringTheory.isSuffix_def;
+val isSuffix_side_def = definition"issuffix_side_def";
+val isSuffix_thm = Q.prove (
+  `!s1 s2. issuffix_side s1 s2`,
+  rw[isSuffix_side_def, isStringThere_aux_side_thm] ) |> update_precondition
+
+val _ = next_ml_names := ["isPrefix"];
+val result = translate mlstringTheory.isPrefix_def;
+val isPrefix_side_def = definition"isprefix_side_def";
+val isPrefix_thm = Q.prove (
+  `!s1 s2. isprefix_side s1 s2`,
+  rw[isPrefix_side_def, isStringThere_aux_side_thm] ) |> update_precondition
+
+val _ = ml_prog_update open_local_block;
+val result = translate mlstringTheory.compare_aux_def;
+val compare_aux_side_def = theorem"compare_aux_side_def";
+val _ = ml_prog_update open_local_in_block;
+
+val _ = next_ml_names := ["compare"];
+val result = translate mlstringTheory.compare_def;
+val compare_side_def = definition"compare_side_def";
+
+val compare_aux_side_thm = Q.prove (
+  `!s1 s2 ord n len. (n + len =
+    if strlen s1 < strlen s2
+      then strlen s1
+    else strlen s2) ==> compare_aux_side s1 s2 ord n len`,
+  Induct_on `len` \\ rw [Once compare_aux_side_def]);
+
+val compare_side_thm = Q.prove (
+  `!s1 s2. compare_side s1 s2`,
+  rw [compare_side_def, compare_aux_side_thm] ) |> update_precondition
+
+val _ = next_ml_names := ["<"];
+val _ = translate mlstringTheory.mlstring_lt_def;
+val _ = next_ml_names := ["<="];
+val _ = translate mlstringTheory.mlstring_le_def;
+val _ = next_ml_names := [">="];
+val _ = translate mlstringTheory.mlstring_ge_def;
+val _ = next_ml_names := [">"];
+val _ = translate mlstringTheory.mlstring_gt_def;
+
+val _ = ml_prog_update open_local_block;
+val result = translate mlstringTheory.collate_aux_def;
+val collate_aux_side_def = theorem"collate_aux_side_def";
+val _ = ml_prog_update open_local_in_block;
+
+val _ = next_ml_names := ["collate"];
+val result = translate mlstringTheory.collate_def;
+val collate_side_def = definition"collate_side_def";
+
+val collate_aux_side_thm = Q.prove (
+  `!f s1 s2 ord n len. (n + len =
+    if strlen s1 < strlen s2
+      then strlen s1
+    else strlen s2) ==> collate_aux_side f s1 s2 ord n len`,
+  Induct_on `len` \\ rw [Once collate_aux_side_def]);
+
+val collate_side_thm = Q.prove (
+  `!f s1 s2. collate_side f s1 s2`,
+  rw [collate_side_def, collate_aux_side_thm] ) |> update_precondition
+
+val _ = ml_prog_update close_local_blocks;
+
+
 val _ = export_theory();
